src/Init/Prelude.lean
@@ -2568,17 +2568,17 @@ structure Array (α : Type u) where
   /--
   Converts a `Array α` into an `List α`.
 
-  At runtime, this projection is implemented by `Array.toList` and is O(n) in the length of the
+  At runtime, this projection is implemented by `Array.toListImpl` and is O(n) in the length of the
   array. -/
-  data : List α
+  toList : List α
 
-attribute [extern "lean_array_data"] Array.data
+attribute [extern "lean_array_to_list"] Array.toList
 attribute [extern "lean_array_mk"] Array.mk
 
 /-- Construct a new empty array with initial capacity `c`. -/
 @[extern "lean_mk_empty_array_with_capacity"]
 def Array.mkEmpty {α : Type u} (c : @& Nat) : Array α where
-  data := List.nil
+  toList := List.nil
 
 /-- Construct a new empty array. -/
 def Array.empty {α : Type u} : Array α := mkEmpty 0
@@ -2586,12 +2586,12 @@ def Array.empty {α : Type u} : Array α := mkEmpty 0
 /-- Get the size of an array. This is a cached value, so it is O(1) to access. -/
 @[reducible, extern "lean_array_get_size"]
 def Array.size {α : Type u} (a : @& Array α) : Nat :=
- a.data.length
+ a.toList.length
 
 /-- Access an element from an array without bounds checks, using a `Fin` index. -/
 @[extern "lean_array_fget"]
 def Array.get {α : Type u} (a : @& Array α) (i : @& Fin a.size) : α :=
-  a.data.get i
+  a.toList.get i
 
 /-- Access an element from an array, or return `v₀` if the index is out of bounds. -/
 @[inline] abbrev Array.getD (a : Array α) (i : Nat) (v₀ : α) : α :=
@@ -2608,7 +2608,7 @@ Push an element onto the end of an array. This is amortized O(1) because
 -/
 @[extern "lean_array_push"]
 def Array.push {α : Type u} (a : Array α) (v : α) : Array α where
-  data := List.concat a.data v
+  toList := List.concat a.toList v
 
 /-- Create array `#[]` -/
 def Array.mkArray0 {α : Type u} : Array α :=
@@ -2654,7 +2654,7 @@ count of 1 when called.
 -/
 @[extern "lean_array_fset"]
 def Array.set (a : Array α) (i : @& Fin a.size) (v : α) : Array α where
-  data := a.data.set i.val v
+  toList := a.toList.set i.val v
 
 /--
 Set an element in an array, or do nothing if the index is out of bounds.
